rocq/theories/TypeSystem/AssocTypingFacts.v
@@ -28,3 +28,29 @@ Proof.
   - constructor.
   - simpl. econstructor; eauto.
 Qed.
+
+Lemma typed_args_assoc_checked_same_bindings :
+  forall env fenv Ω n Γ args ps Γ',
+    typed_args_assoc_checked env fenv Ω n Γ args ps Γ' ->
+    ctx_same_bindings Γ Γ'.
+Proof.
+  intros env fenv Ω n Γ args ps Γ' Hargs.
+  induction Hargs.
+  - apply ctx_same_bindings_refl.
+  - eapply ctx_same_bindings_trans.
+    + destruct typed_same_bindings as [Htyped _].
+      eapply Htyped. exact H.
+    + exact IHHargs.
+Qed.
+
+Lemma typed_args_assoc_checked_params_of_tys_map_param_ty :
+  forall env fenv Ω n Γ args ps Γ',
+    typed_args_assoc_checked env fenv Ω n Γ args ps Γ' ->
+    typed_args_assoc_checked env fenv Ω n Γ args
+      (params_of_tys (map param_ty ps)) Γ'.
+Proof.
+  intros env fenv Ω n Γ args ps Γ' Hargs.
+  induction Hargs.
+  - constructor.
+  - simpl. econstructor; eauto.
+Qed.
